

Sunday, 11 January 2026 12:42 PM

②  $\theta = \pi/2$ , Equatorial plane ( $\theta = \pi/2$ ).

Schwarzschild line element is,

$$ds^2 = - \left(1 - \frac{2M}{r}\right) dt^2 + \left(1 - \frac{2M}{r}\right)^{-1} dr^2 + r^2 d\phi^2$$

$\tau \rightarrow$  Achilles' proper time

$$\mathcal{L} = \frac{1}{2} g_{\mu\nu} \dot{z}^\mu \dot{z}^\nu \quad \text{where } \dot{z} = \frac{dz}{d\tau}$$

In general relativity, motion of a free falling particle is given by geodesic. We can describe this motion using a Lagrangian  $\mathcal{L}$ .

From provided Schwarzschild metric, non zero components of the metric tensor  $g_{\mu\nu}$  are:

$$g_{tt} = - \left(1 - \frac{2M}{r}\right) \quad g_{\phi\phi} = r^2$$

$$g_{rr} = \left(1 - \frac{2M}{r}\right)^{-1}$$

Substituting these into the given Lagrangian formula,

$$\mathcal{L} = \frac{1}{2} \left[ - \left(1 - \frac{2M}{r}\right) \dot{t}^2 + \left(1 - \frac{2M}{r}\right)^{-1} \dot{r}^2 + r^2 \dot{\phi}^2 \right]$$

$\rightarrow$  A coordinate  $x^\alpha$  is said to be cyclic if the Lagrangian does not explicitly depend on it.  $\left( \frac{\partial \mathcal{L}}{\partial x^\alpha} = 0 \right)$

• Time ( $t$ )  $\rightarrow$  only appears as a derivative

$\dot{t}$ . There is no  $t$  term on its own,

$\therefore$   $t$  is cyclic

• Azimuthal angle ( $\phi$ ):  $\phi$  only appears as  $\dot{\phi}$ .

No  $\phi$  term on its own.

$\therefore \phi$  is cyclic

...  $\square$  ...

→ According to **Noether's theorem**, every cyclic coordinate corresponds to a conserved quantity.

- Canonical momentum  $p_\alpha$  is defined as:

$$p_\alpha = \frac{\partial \mathcal{L}}{\partial \dot{x}^\alpha}$$

for the time coordinate ( $t$ ):

$$p_t = \frac{\partial \mathcal{L}}{\partial \dot{t}} = \frac{1}{2} \left[ -2 \left( 1 - \frac{2M}{r} \right) \dot{t} \right] = - \left( 1 - \frac{2M}{r} \right) \dot{t}$$

This is associated with energy of the particle at infinity.

By convention,

$$E \equiv -p_t = \left( 1 - \frac{2M}{r} \right) \dot{t}$$

for angular coordinate ( $\phi$ ):

$$p_\phi = \frac{\partial \mathcal{L}}{\partial \dot{\phi}} = \frac{1}{2} \left[ 2r^2 \dot{\phi} \right] = r^2 \dot{\phi}$$

∴ This is the Angular Momentum ( $L$ ) of the particle:  $L \equiv p_\phi = r^2 \dot{\phi}$

→ Why equatorial plane can be taken?

- Spherical symmetry of the Schwarzschild metric means that the mass does not prefer any specific direction
- In a central potential, motion of particles is confined to a single plane.
- Thus, we are free to rotate our plane of motion so that it aligns with the equatorial plane.

⑥ Normalization conditions

$$\rightarrow g_{\mu\nu} \dot{x}^\mu \dot{x}^\nu = -1$$

Using Schwarzschild metric for equatorial plane, ( $\theta = \pi/2$ ),

we expand  $g_{\mu\nu} \dot{x}^\mu \dot{x}^\nu = -1$

$$\Rightarrow g_{tt} \dot{t}^2 + g_{rr} \dot{r}^2 + g_{\phi\phi} \dot{\phi}^2 = -1$$

$$\Rightarrow - \left(1 - \frac{2M}{r}\right) \dot{t}^2 + \left(1 - \frac{2M}{r}\right)^{-1} \dot{r}^2 + r^2 \dot{\phi}^2 = -1$$

from part (a)  $\rightarrow \dot{t} = \frac{E}{1 - \frac{2M}{r}} \rightarrow \dot{\phi} = \frac{L}{r^2}$

$$- \left(1 - \frac{2M}{r}\right) \left[ \frac{E}{1 - \frac{2M}{r}} \right]^2 + \left(1 - \frac{2M}{r}\right)^{-1} \dot{r}^2 + r^2 \left[ \frac{L}{r^2} \right]^2 = -1$$

$$\Rightarrow - \frac{E^2}{\left(1 - \frac{2M}{r}\right)} + \frac{\dot{r}^2}{\left(1 - \frac{2M}{r}\right)} + \frac{L^2}{r^2} = -1$$

$\Rightarrow$  Multiplying entire equation by  $\left(1 - \frac{2M}{r}\right)$

$$\Rightarrow -E^2 + \dot{r}^2 + \frac{L^2}{r^2} \left(1 - \frac{2M}{r}\right) = -\left(1 - \frac{2M}{r}\right)$$

$$\Rightarrow \left(1 - \frac{2M}{r}\right) + \frac{L^2}{r^2} \left(1 - \frac{2M}{r}\right) + \dot{r}^2 = E^2$$

$$\Rightarrow \left(1 - \frac{2M}{r}\right) \left(1 + \frac{L^2}{r^2}\right) + \dot{r}^2 = E^2 \quad \text{--- (I)}$$

Given radial form  $\Rightarrow \dot{r}^2 + V^2(r) = E^2$  --- (II)

Comparing (I) and (II),

$$\boxed{V^2(r) = \left(1 - \frac{2M}{r}\right) \left(1 + \frac{L^2}{r^2}\right)} \rightarrow \text{hence, proven.}$$

② Specialize to  $L=0$ .

Spaceship starts from rest at  $r=R$ .

radial velocity at starting point,  $\dot{r}=0$

$\therefore L=0, \dot{r}=0, r=R$  in our radial

equation,  $\dot{r}^2 + V^2(r) = E^2$

$$0^2 + \left(1 - \frac{2M}{R}\right) \left(1 + \frac{0^2}{R^2}\right) = E^2$$

$$\Rightarrow \boxed{E^2 = \left(1 - \frac{2M}{R}\right)} \quad \text{--- (iii)}$$

Now, again,

$$\dot{r}^2 + \left(1 - \frac{2M}{r}\right) \left(1 + \frac{L^2}{R^2}\right) = E^2$$

Here,  $r$  changes but  $L=0$ ,

$$\dot{r}^2 + \left(1 - \frac{2M}{r}\right) (1+0) = E^2$$

Substituting, (iii)

$$\Rightarrow \dot{r}^2 + \left(1 - \frac{2M}{r}\right) = \left(1 - \frac{2M}{R}\right)$$

$$\Rightarrow \boxed{\dot{r}^2 = 2M \left( \frac{1}{r} - \frac{1}{R} \right)}$$

$$\frac{dr}{d\tau} = - \sqrt{2M \left( \frac{1}{r} - \frac{1}{R} \right)}$$

→ Achilles is starting from a high point  $r=R$  and its radial distance decreases to 0.

$\therefore$  We take the negative sign.

$$r = \frac{R}{2} (1 + \cos x) \quad \text{when } x = 0$$

$$r = R$$

$$\text{when } x = \pi,$$

$$r = 0.$$

$$\Rightarrow \frac{dr}{dx} = -\frac{R}{2} \sin x$$

$$\frac{dr}{dz} = \frac{dr}{dx} \frac{dx}{dz}$$

$r(x)$  into  $r^2$  equation,

$$\left( \frac{dr}{dx} \cdot \dot{x} \right)^2 = 2M \left( \frac{2}{R(1+\cos x)} - \frac{1}{R} \right)$$

$$\Rightarrow \left( -\frac{R}{2} \sin x \cdot \dot{x} \right)^2 = 2M \left( \frac{2}{R(1+\cos(\frac{x}{2}))} - \frac{1}{R} \right)$$

$$\Rightarrow \left( \frac{R^2}{4} \sin^2 x \cdot (\dot{x})^2 \right) = \frac{2M}{R} \left( \frac{1 - \cos^2(x/2)}{\cos^2(x/2)} \right)$$

$$\Rightarrow \frac{R^2}{4} \sin^2 x \cdot \left( \frac{dx}{dz} \right)^2 = \frac{2M}{R} \left( \frac{\sin^2(x/2)}{\cos^2(x/2)} \right)$$

$$\Rightarrow \frac{R^2}{4} \sin^2 x \left( \frac{dx}{dz} \right)^2 = \frac{2M}{R} \tan^2(x/2)$$

$$\Rightarrow \frac{R^3}{8} \left( \frac{dx}{dz} \right)^2 \sin^2 x = M \tan^2(x/2)$$

$$\Rightarrow \frac{R^3}{8M} \left( \frac{dx}{dz} \right)^2 \cancel{4 \sin^2 \frac{x}{2} \cos^2 \frac{x}{2}} = \frac{\sin^2(x/2)}{\cos^2(x/2)}$$

$$\Rightarrow \frac{R^3}{8M} \left( \frac{dx}{d\tau} \right)^2 = \frac{1}{4\cos^4(x/2)}$$

$$\Rightarrow \frac{R^3}{8M} \times 4\cos^4(x/2) = (d\tau)^2$$

$$\Rightarrow \frac{R^3}{8M} (2\cos^2(x/2))^2 (dx)^2 = (d\tau)^2$$

$$\Rightarrow \frac{R^3}{8M} (1+\cos x)^2 (dx)^2 = (d\tau)^2$$

$$\Rightarrow \sqrt{\frac{R^3}{8M}} (1+\cos x) dx = d\tau$$

$\Rightarrow$  Integrating both sides,

$$\int_0^x \frac{R^{3/2}}{2\sqrt{2M}} (1+\cos x) dx = \int_0^\tau d\tau$$

$$\Rightarrow \frac{R^{3/2}}{2\sqrt{2M}} (x + \sin x) = \tau(x)$$

At  $\tau=0$ ,  $\cos x = -1 \rightarrow x = \pi$

$\Rightarrow$  At  $x = \pi$

$$\tau_{\text{total}} = \frac{R^{3/2}}{2\sqrt{2M}} (\pi + \sin \pi)$$

$$\Rightarrow \frac{R^{3/2}}{2\sqrt{2M}}$$

$$C_{\text{total}} = \frac{\pi K}{2\sqrt{2M}}$$

$$\textcircled{a} \quad \frac{dr}{dt} = \frac{dr/d\tau}{dt/d\tau} = \frac{\dot{r}}{\dot{t}}$$

we know from previous parts,

$$E = \left(1 - \frac{2M}{r}\right) \dot{t}$$

$$\Rightarrow \dot{t} = \frac{E}{1 - \frac{2M}{r}} \longrightarrow \frac{dr}{dt} = \frac{\dot{r}}{\frac{E}{1 - \frac{2M}{r}}}$$

$$\therefore \frac{dr}{dt} = \frac{\dot{r}}{E} \left(1 - \frac{2M}{r}\right)$$

$$\Rightarrow \frac{dr}{dt} = \frac{\left(1 - \frac{2M}{r}\right) \dot{r}}{E}$$

\* Tortoise Coordinate

$$r_* = r + 2M \ln \left| \frac{r}{2M} - 1 \right|$$

$$\frac{dr_*}{dr} = 1 + \frac{2M}{\left(\frac{r}{2M} - 1\right)} \times \frac{1}{2M} = 1 + \frac{1}{\frac{r}{2M} - 1}$$

$$\Rightarrow \frac{\frac{r}{2M} - 1 + 1}{\frac{r}{2M} - 1} = \frac{\frac{r}{2M}}{\frac{r}{2M} - 1} = \left(\frac{r - 2M}{r}\right)^{-1} = \left(1 - \frac{2M}{r}\right)^{-1}$$

$$\frac{dr_*}{dt} = \frac{dr}{dt} \cdot \frac{dt}{dr} \Rightarrow \left(1 - \frac{2M}{r}\right)^{-1} \left(1 - \frac{2M}{r}\right) \cdot \frac{\dot{r}}{E}$$

$$\therefore \frac{dr_*}{dt} = \frac{\dot{r}}{E}$$

$$V^2(r) = \left(1 - \frac{2M}{r}\right) \left(1 + \frac{L^2}{r^2}\right)$$

$\Rightarrow$  As Achilles goes to event horizon,  $(r \rightarrow 2M^+)$

$$\Rightarrow V^2(r) \rightarrow 0$$

From radial equation,  $\dot{r}^2 = E^2 - V^2(r)$

$\Rightarrow$  Since  $V^2(r) \rightarrow 0$  as  $r \rightarrow 2M^+$

$$\therefore \dot{r}^2 \approx E^2 \Rightarrow \boxed{\dot{r} \approx -E}$$

$\rightarrow$  we choose negative root because Achilles is falling in.

$$\dot{r} \approx -E \rightarrow \boxed{\frac{dr_*}{dt} \approx -\frac{E}{E} = -1}$$

Integrating,

$$r_* \approx -t + k \quad \text{where } k \rightarrow \text{constant}$$

$$r_* = r + 2M \ln \left| \frac{r}{2M} - 1 \right|$$

As  $r \rightarrow 2M$  logarithmic term dominates,

$$\text{Approximating, } \Rightarrow r \approx 2M \ln \left| \frac{r}{2M} - 1 \right|$$

$$\therefore 2M \ln \left| \frac{r}{2M} - 1 \right| \approx -t + k$$

$$\Rightarrow \ln \left| \frac{r}{2M} - 1 \right| \approx \frac{-t}{2M} + \frac{k}{2M}$$

$$\Rightarrow \frac{r}{2M} - 1 \approx e^{-t/2M} \cdot e^{k/2M}$$

$$\Rightarrow r - 2M \approx 2M e^{-t/2M} \cdot e^{k/2M}$$

$$\Rightarrow r \approx C e^{-t/2M} + 2M$$

→ To convert  $-t/2M$  to seconds, replace  $2M$  with Schwarzschild radius,  $R_s = \frac{2GM}{c^2}$

© Does Achilles reach the tortoise in finite Schwarzschild time?

- No. As derived in part ①,  $r(t) \approx C e^{-t/2M} + 2M$

$\therefore e^{-t/2M} \rightarrow 0$  as  $t \rightarrow \infty$  which implies,

$$r(t) \approx 2M \text{ as } t \rightarrow \infty.$$

Resolving this paradox, the two explanations

are both physically valid yet different

are both physically valid, yet different because they represent different observers, Achilles as one and the tortoise as the other

- Achilles sees that it reaches the tortoise in finite proper time.
  - Tortoise never sees Achilles cross the horizon because the signals take infinite coordinate time to reach it.
- Another point to be noted is that we are deriving conclusions only on the basis of the mathematical equations, we have solved and the topics at hand are a part of general relativity which is highly variable.